CompCert/cfrontend/Locally.v
@@ -22,19 +22,37 @@ Ltac unfold_locally :=
   inversion H1 as (H4&H5); inv H5; clear H4; clear H1; clear H0;
   rewrite heap_union_empty_l | rewrite heap_union_empty_r; auto].
 
-Lemma locally_indep {A} : forall (P : iProp) (le : t A), ⊢P -∗ locally le (fun _ => P).
+Lemma locally_base {A} : forall (le : t A), ⊢ locally le (fun le' => emp).
 Proof.
-  unfold_locally. intros. apply H2.
+  unfold locally; unfold hlocally; MonPred.unseal; split; MonPred.unseal; intros i h H.
+  intros. inv H.  inv H2. red. split; auto. reflexivity.
 Qed.
 
-Lemma locally_simpl {A} : forall P (le : t A), ⊢(∀ le', P le') -∗ locally le (fun le' => P le').
-Proof.
-  unfold_locally. intros. apply H2.
-Qed.
-
-Lemma locally_delete {A} : forall P (le : t A), ⊢ locally le (fun le' => P le') -∗ P le.
+Lemma locally_elim {A} : forall P (le : t A), ⊢ locally le (fun le' => P le') -∗ P le.
 Proof.
   unfold_locally. apply H2. eauto. 
+Qed.
+
+Lemma locally_consequence {A} : forall (P Q : t A -> iProp) (le : t A),
+    ⊢locally le (λ le', P le') -∗ (∀ le, P le -∗ Q le) -∗ locally le (λ le', Q le').
+Proof.
+  unfold_locally. clear H3. intros j H. destruct j. clear H.
+  repeat red. exists (hheap_ctx h1), h1, heap_empty. repeat split; auto with heap_scope.
+  red. intros. inversion_star h P. clear H. red in P1. subst.
+  edestruct P2. instantiate (1 := tt). repeat red. exists heap_empty, h0.
+  repeat split; auto with heap_scope.
+  apply map_disjoint_empty_l. rewrite heap_union_empty_l; auto. inversion_star h P.
+  clear H. destruct P4. inv H1. clear P5.
+  rewrite heap_union_empty_r. rewrite heap_union_empty_r in P3. rewrite heap_union_empty_r in H0.
+  apply H. exists h, h1. repeat split; auto. apply H2. intros. erewrite <- H0; auto.
+  eapply lookup_union_Some; eauto. apply heap_union_comm; auto. apply map_disjoint_empty_r.
+  rewrite heap_union_empty_r; auto.
+Qed.
+
+Lemma locally_consequence_2 {A} : forall P Q (le : t A),
+    ⊢ (∀ le, P le -∗ Q le) -∗ locally le (λ le', P le') -∗ locally le (λ le', Q le').
+Proof.
+  iIntros "* HA HB". iApply (locally_consequence with "HB HA"); eauto.
 Qed.
 
 Lemma locally_sep {A} : forall P R (le : t A),
@@ -51,6 +69,7 @@ Proof.
   rewrite heap_union_empty_r; auto. 
 Qed.
 
+
 Lemma locally_and {A} : forall P R (le : t A),
     ⊢locally le (fun le' => P le') ∧ locally le (fun le' => R le') -∗
             locally le (fun le' => P le' ∧ R le').
@@ -65,37 +84,36 @@ Proof.
       rewrite heap_union_empty_l in H0. apply (H _ H0). apply (H1 _ H0).
 Qed.
 
-Lemma locally_and_out {A} : forall P R (le : t A),
+Lemma locally_and_2 {A} : forall P R (le : t A),
     ⊢locally le (fun le' => P le' ∧ R le') -∗
      locally le (fun le' => P le') ∧ locally le (fun le' => R le').
 Proof.
   unfold locally; unfold hlocally; MonPred.unseal; split; MonPred.unseal; intros i h H;
   destruct i; inversion H as (H0&H1); clear H; inv H1;
   clear H0; intros j H; destruct j; clear H.
-  exists emp, heap_empty, heap_empty; repeat split; auto.
+  exists emp, heap_empty, heap_empty. repeat split; auto.
   3 : rewrite heap_union_empty_l; auto.
   all : inversion_star h P; clear H;
     intros; inv P1; inv H1; clear H0; clear P3; rewrite heap_union_empty_l;
       rewrite heap_union_empty_l in H; eapply P2 in H; destruct H; auto.
 Qed.
 
+Lemma locally_simpl {A} : forall P (le : t A), ⊢(∀ le', P le') -∗ locally le (fun le' => P le').
+Proof.
+  iIntros "* HA". iApply locally_consequence. iApply locally_base. iIntros "* _". iApply "HA".
+Qed.
+  
+Lemma locally_indep {A} : forall (P : iProp) (le : t A), ⊢P -∗ locally le (fun _ => P).
+Proof.
+  iIntros. iApply locally_simpl. auto.
+Qed.
+
 
 Lemma locally_indep_frame {A} : forall P R (Q : iProp) (le : t A),
     ⊢locally le (fun le' => P le' -∗ R le') -∗ locally le (fun le' => P le' ∗ Q -∗ R le' ∗ Q).
 Proof.
-  unfold_locally. intros. repeat red. repeat red in H2.
-  intros. destruct a. eapply H2 in H; eauto. clear H0.
-  destruct H. inversion_star h P. clear H. destruct P2.
-  inv H0. clear P3. red in H. rewrite heap_union_empty_r.
-  exists x. exists h,heap_empty. repeat split; auto with heap_scope. intros h0 P3. inversion_star h P.
-  clear P3. inversion_star h P. clear P4. eexists. exists h4.
-  repeat split; auto. eapply H. exists h1, h3. repeat split; auto.
-  - subst. eapply heap_disjoint_union_r_l; eauto.
-  - subst. apply map_disjoint_union_l. split; auto.
-    apply map_disjoint_union_r in P5 as (_&P10). auto.
-  - subst. apply heap_union_assoc.
-  - apply map_disjoint_empty_r.
-  - rewrite heap_union_empty_r; auto.
+  iIntros "* HA". iApply locally_consequence_2; eauto.
+  iIntros "* HA [HB $]". iApply ("HA" with "HB").
 Qed.
 
 Lemma locally_modout {A} : forall P (le : t A),
@@ -106,6 +124,13 @@ Proof.
   eapply lookup_union_Some; eauto.
 Qed.
 
+Lemma locally_idempotence {A} : forall P (le : t A),
+    ⊢locally le (fun le' => P le') -∗ locally le (fun le' => locally le' (fun le'' => P le'')).
+Proof.
+  unfold_locally. intros. apply H2. intros.
+  pose H1. apply H in e.
+  etransitivity; eauto.
+Qed.
 
 Lemma locally_sep_indep_r {A} : forall P Q (le : t A),
     ⊢locally le (fun le' => P le') ∗ Q -∗ locally le (fun le' => P le' ∗ Q).
@@ -125,18 +150,17 @@ Proof.
   unfold_locally. red. intros. red in H2. apply H2. apply H.
 Qed.
 
-Lemma locally_doublon {A} : forall P (le : t A),
-    ⊢locally le (fun le' => P le') -∗ locally le (fun le' => locally le' (fun le'' => P le'')).
+Lemma locally_exists' {A B} : forall P (le : t A), 
+      ⊢(∃ t, locally le (fun le' => P t le')) -∗ locally le (fun le' => ∃ (t : B), P t le').
 Proof.
-  unfold_locally. intros. apply H2. intros.
-  pose H1. apply H in e.
-  etransitivity; eauto.
+  unfold_locally. intros. clear H3. destruct H2. repeat red. exists x.
+  apply H0 in H. apply H.
 Qed.
-
+  
 Lemma locally_exists {A B} : forall P (le : t A), ∀ t,
       ⊢locally le (fun le' => P t le') -∗ locally le (fun le' => ∃ (t : B), P t le').
 Proof.
-  unfold_locally. intros. apply H2 in H. exists t0. apply H.
+  iIntros. iApply locally_exists'. iExists t0. iFrame.
 Qed.
 
 Lemma locally_exists_sep {A B} : forall P Q (le : t A), ∀ t,
@@ -146,38 +170,14 @@ Proof.
   iIntros "* HA HB". iApply locally_exists. iApply (locally_sep with "HA HB").
 Qed.
 
-Lemma locally_apply {A} : forall (P Q : t A -> iProp) (le : t A),
-    ⊢locally le (λ le', P le') -∗ (∀ le, P le -∗ Q le) -∗ locally le (λ le', Q le').
-Proof.
-  unfold_locally. clear H3. intros j H. destruct j. clear H.
-  repeat red. exists (hheap_ctx h1), h1, heap_empty. repeat split; auto with heap_scope.
-  red. intros. inversion_star h P. clear H. red in P1. subst.
-  edestruct P2. instantiate (1 := tt). repeat red. exists heap_empty, h0.
-  repeat split; auto with heap_scope.
-  apply map_disjoint_empty_l. rewrite heap_union_empty_l; auto. inversion_star h P.
-  clear H. destruct P4. inv H1. clear P5.
-  rewrite heap_union_empty_r. rewrite heap_union_empty_r in P3. rewrite heap_union_empty_r in H0.
-  apply H. exists h, h1. repeat split; auto. apply H2. intros. erewrite <- H0; auto.
-  eapply lookup_union_Some; eauto. apply heap_union_comm; auto. apply map_disjoint_empty_r.
-  rewrite heap_union_empty_r; auto.
-Qed.
-
-
-Lemma locally_consequence {A} : forall (P Q : t A -> iProp) (le : t A),
-    ⊢(∀ le, P le -∗ Q le) -∗ locally le (λ le', P le') -∗ locally le (λ le', Q le').
-Proof.
-  iIntros "* HA HB". iApply (locally_apply with "HB HA").
-Qed.
-
-    
 Lemma locally_delete_2 {A} : forall P Q R (le : t A),
-      ⊢locally le (fun le' => R le') -∗
-      locally le (fun le' => P le') -∗
-      (∀ le, R le -∗ P le -∗ Q le) -∗
-      locally le (fun le' => Q le').
+    ⊢locally le (fun le' => R le') -∗
+     locally le (fun le' => P le') -∗
+     (∀ le, R le -∗ P le -∗ Q le) -∗
+     locally le (fun le' => Q le').
 Proof.
   iIntros "* HA HB HC". iDestruct (locally_sep with "HA HB") as "HA".
-  iApply (locally_apply with "HA [HC]"). iIntros "* [HA HB]".
+  iApply (locally_consequence with "HA [HC]"). iIntros "* [HA HB]".
   iApply ("HC" with "HA HB").
 Qed.
 
@@ -190,9 +190,7 @@ Lemma locally_delete_3 {A} : forall P Q R S (le : t A),
 Proof.
   iIntros "* HA HB HC HD". iDestruct (locally_sep with "HB HC") as "HB".
   iApply (locally_delete_2 with "HA HB"). iIntros "* HA [HB HC]". iApply ("HD" with "HA HB HC").
-Qed.
-  
-  
+Qed.  
 
 Lemma locally_conseq {A} : forall P Q Q' (le : t A),
     ⊢locally le (fun le' => P le' -∗ Q le') -∗
@@ -216,7 +214,7 @@ Proof.
 Qed.
 
 Lemma locally_set {A} : forall Q (le : t A) t v,
-    ⊢\s t -∗ locally le (fun le' => Q le') -∗ locally (set t v le) (fun le' => Q le') ∗ \s t.
+    ⊢IsFresh t -∗ locally le (fun le' => Q le') -∗ locally (set t v le) (fun le' => Q le') ∗ IsFresh t.
 Proof.
   unfold_locally.
   destruct H2. red in H. clear H3. repeat red. intros. destruct a. clear H0.
@@ -233,24 +231,19 @@ Qed.
 Lemma locally_out {A} : forall P Q (le : t A),
     ⊢locally le (fun le' => P le' -∗ Q le') -∗ P le -∗ Q le.
 Proof.
-  iIntros "* HA HB". iDestruct (locally_delete with "HA HB") as "HA". iApply "HA".
+  iIntros "* HA HB". iDestruct (locally_elim with "HA HB") as "HA". iApply "HA".
 Qed.
 
 Lemma locally_conseq_pure {A} : forall (P Q : t A -> Prop) (le : t A),
     (forall le, P le -> Q le) -> ⊢locally le (λ le', ⌜ P le' ⌝) -∗ locally le (λ le', ⌜ Q le' ⌝).
 Proof.
-  intros. iApply locally_consequence. eauto.
+  intros. iApply locally_consequence_2. eauto.
 Qed.
 
-Lemma locally_destruct {A} : forall Q (le : t A) t,
-    ⊢locally le (fun le' => \s t ∗ Q le') -∗ locally le (fun le' => (\s t -∗ \s t ∗ Q le') ∗ \s t).
+Lemma locally_destruct {A} : forall Q (le : t A) P,
+    ⊢locally le (fun le' => P ∗ Q le') -∗ locally le (fun le' => (P -∗ P ∗ Q le') ∗ P).
 Proof.
-  unfold_locally. clear H3. repeat red. intros.
-  eapply H2 in H. inversion_star h P. clear H. destruct P0. red in H.
-  exists h0, h. subst. repeat split; auto. repeat red. intros. clear H. destruct a.
-  exists (hheap_ctx h0), h0, heap_empty. repeat split; auto with heap_scope. intros h H.
-  inversion_star h P. clear H. red in P0. destruct P3. red in H. exists h2, h1.
-  subst. repeat split; auto. exists x0. reflexivity. apply heap_union_comm; auto.
-  apply map_disjoint_empty_r. rewrite heap_union_empty_r; auto.
-  exists x. reflexivity. apply heap_union_comm; auto.
+  iIntros "* HA".
+  iApply (locally_consequence with "HA"). iIntros "* [HA HB]". iSplitR "HA"; auto.
+  iIntros "$ //". 
 Qed.
